verif/indices/verif_BtreeIndexASI.v
@@ -4,16 +4,9 @@ Require Import VST.floyd.VSU_addmain.
 Require Import indices.spec_BtreeIndexASI.
 Require Import indices.btree_instance.
 Require Import indices.btree_wrappers.
+Require Import indices.verif_BtreeASI.
 
 Require Import btrees.relation_mem.
-Require Import btrees.btrees_spec.
-Require Import btrees.verif_newrel.
-Require Import btrees.verif_newcursor.
-Require Import btrees.verif_gotokey.
-Require Import btrees.verif_getrecord.
-Require Import btrees.verif_putrecord.
-Require Import btrees.verif_movetonext.
-Require Import btrees.verif_movetoprev.
 
 Instance BtreeIndexCompSpecs : compspecs. make_compspecs prog. Defined.
 
@@ -21,288 +14,68 @@ Section BtreeIndex_Component.
 
 Definition BtreeIndexVprog : varspecs. mk_varspecs prog. Defined.
 
-Definition BI_ASI: funspecs := BtreeIndexASI.
+ Definition internal_specs: funspecs := btrees_spec.all_specs.
 
-Definition spec_gprog: funspecs := btrees_spec.Gprog.
-Definition wrap_gprog: funspecs := btree_wrappers.Gprog.
+Definition imported_specs: funspecs := [ (_malloc, library.malloc_spec'); (_free, library.free_spec'); 
+    (_exit, library.exit_spec') ].
 
-Definition internal_specs: funspecs := G_merge spec_gprog wrap_gprog.
-
-Definition imported_specs := [currNode_spec].
-
-Definition BtreeIndexGprog:funspecs := (* imported_specs ++ *) internal_specs.
-
-Lemma gprog_app_sub:  forall V G1 G2 f spec, 
-  list_norepet (map fst G2) -> 
-  list_norepet (map fst V ++ map fst (G1 ++ G2)) ->
-  semax_body V G2 f spec -> 
-  semax_body V (G1 ++ G2) f spec.
-Proof. 
-  intros. eapply semax_body_subsumption; eauto.
-  apply tycontext_sub_Gprog_app2; auto.
-Qed.
-
-Lemma gprog_gmerge_sub: forall V G1 G2 f spec, 
-  list_norepet (map fst G2) -> 
-  list_norepet (map fst V ++ map fst (G_merge G1 G2)) ->
-  semax_body V G2 f spec -> 
-  semax_body V (G_merge G1 G2) f spec.
-Proof. Admitted.
-
-
-Lemma list_norepet_spec_gprog: 
-  list_norepet (map fst spec_gprog).
-Proof. Admitted.
-
-Lemma list_norepet_vprog:
-  list_norepet (map fst BtreeIndexVprog).
-Proof. Admitted.
-
-
-Lemma list_norepet_wrap_gprog: 
-    list_norepet (map fst wrap_gprog).
-Proof. Admitted. 
-
-Lemma list_disjoint_vprog_gprog:
-  list_disjoint (map fst BtreeIndexVprog) (map fst (G_merge spec_gprog wrap_gprog)).
-Proof. Admitted.
-
-Lemma g_merge_comm: forall G1 G2, 
-  G_merge G1 G2 = G_merge G2 G1.
-Proof. Admitted.
-
-Lemma gprog_wrap_sub: forall f s,
-  semax_body BtreeIndexVprog wrap_gprog f s ->
-  semax_body BtreeIndexVprog BtreeIndexGprog f s.
-Proof.
-  intros. apply gprog_gmerge_sub; auto.
-  apply list_norepet_wrap_gprog.
-  apply list_norepet_append.
-  apply list_norepet_vprog.
-  apply G_merge_LNR.
-  apply list_norepet_spec_gprog.
-  apply list_norepet_wrap_gprog.
-  apply list_disjoint_vprog_gprog.
-Qed.
-
-Lemma gprog_spec_sub: forall f s,
-  semax_body BtreeIndexVprog spec_gprog f s ->
-  semax_body BtreeIndexVprog BtreeIndexGprog f s.
-Proof.
-  intros. unfold BtreeIndexGprog. 
-  unfold internal_specs.
-  rewrite g_merge_comm. 
-  apply gprog_gmerge_sub; auto.
-  apply list_norepet_spec_gprog.
-  apply list_norepet_append.
-  apply list_norepet_vprog.
-  apply G_merge_LNR.
-  apply list_norepet_wrap_gprog.
-  apply list_norepet_spec_gprog.
-  rewrite g_merge_comm.
-  apply list_disjoint_vprog_gprog.
-Qed.
-
-Lemma cardinality_verif:
-  semax_body BtreeIndexVprog BtreeIndexGprog f_RL_NumRecords cardinality_funspec.
-Proof.
-  eapply semax_body_funspec_sub. 
-  2: eapply sub_cardinality.
-  apply gprog_wrap_sub.
-  apply body_NumRecords.
-  simpl. 
-  assert (K: list_norepet [_t'1]). 
-  apply list_norepet_cons. 2: apply list_norepet_nil.
-  inversion 1. assert (M: list_norepet[_t'2; _t'1]).
-  apply list_norepet_cons; auto. inversion 1.
-  inversion H0. inversion H0.
-  apply list_norepet_cons; auto. 
-  inversion 1.
-  inversion H0. inversion H0. inversion H1. inversion H1.
-Qed.
+(* this is imported + internal *)
+Definition BtreeIndexGprog:funspecs := imported_specs ++ internal_specs.
 
 Definition BtreeIndexComponent: @Component NullExtension.Espec BtreeIndexVprog _ 
-      nil [] prog [] [].
+      nil imported_specs prog BtreeIndexASI internal_specs.
 Proof.
-  mkComponent. 
-  admit. admit. admit.
-  + solve_SF_internal create_index_verif.
-  + solve_SF_internal newDB_verif.
-  + discriminate.
-  Defined.
-
-
-Lemma create_index_verif:
-  semax_body BtreeIndexVprog BtreeIndexGprog f_RL_NewRelation create_index_funspec.
-Proof. 
-  eapply semax_body_funspec_sub.
-  2: eapply sub_create_index.
-  apply gprog_spec_sub.
-  apply body_NewRelation.
-  simpl.
-  assert (K: list_norepet [_t'1]). 
-  apply list_norepet_cons. 2: apply list_norepet_nil.
-  inversion 1. assert (M: list_norepet[_t'2; _t'1]).
-  apply list_norepet_cons; auto. inversion 1.
-  inversion H0. inversion H0.
-  assert (N: list_norepet [_pNewRelation; _t'2; _t'1]).
-  apply list_norepet_cons; auto. 
-  inversion 1.
-  inversion H0. inversion H0. inversion H1. inversion H1.
-  apply list_norepet_cons; auto.
-  inversion 1. inversion H0. inversion H0.
-  inversion H1. inversion H1. inversion H2. inversion H2.
+  eapply Comp_Exports_sub.
+  eapply BtreeComponent.
+  LNR_tac.
+  inversion 1. repeat if_tac in H1; subst.
+  all: inversion H1; subst; clear H1.
+  + exists (snd btrees_spec.RL_NumRecords_spec).
+      split. auto. apply sub_cardinality.
+  + exists (snd btrees_spec.RL_NewCursor_spec).
+      split. auto. apply sub_create_cursor.
+  + exists (snd btrees_spec.RL_NewRelation_spec).
+      split. auto. apply sub_create_index.
+  + exists (snd btrees_spec.RL_MoveToNext_spec).
+      split. auto. apply sub_move_to_next.
+  + exists (snd btrees_spec.RL_MoveToPrevious_spec).
+      split. auto. apply sub_move_to_previous.
+  + exists (snd btrees_spec.goToKey_spec).
+      split. auto. apply sub_go_to_key.
+  + exists (snd btrees_spec.RL_MoveToFirst_spec).
+      split. auto. apply sub_move_to_first.
+  + exists (snd btrees_spec.RL_GetRecord_spec).
+      split. auto. apply sub_get_record.
+  + exists (snd btrees_spec.RL_PutRecord_spec).
+      split. auto. apply sub_put_record.
 Qed.
 
-
-Lemma create_cursor_verif:
-  semax_body BtreeIndexVprog BtreeIndexGprog f_RL_NewCursor create_cursor_funspec.
-Proof. 
-  eapply semax_body_funspec_sub.
-  2: eapply sub_create_cursor.
-  apply gprog_spec_sub.
-  apply body_NewCursor.
-  simpl.
-  assert (K: list_norepet [_t'2]). 
-  apply list_norepet_cons. 2: apply list_norepet_nil.
-  inversion 1. assert (M: list_norepet[_t'1; _t'2]).
-  apply list_norepet_cons; auto. inversion 1.
-  inversion H0. inversion H0.
-  assert (N: list_norepet [_i; _t'1; _t'2]).
-  apply list_norepet_cons; auto. 
-  inversion 1.
-  inversion H0. inversion H0. inversion H1. inversion H1.
-  assert (O: list_norepet [_cursor; _i; _t'1; _t'2]).
-  apply list_norepet_cons; auto. 
-  inversion 1.
-  inversion H0. inversion H0. inversion H1. inversion H1.
-  inversion H2. inversion H2.
-  apply list_norepet_cons; auto.
-  inversion 1. inversion H0. inversion H0.
-  inversion H1. inversion H1. inversion H2. inversion H2.
-  inversion H3. inversion H3.
-Qed.
-
-(*
-Lemma move_to_next_verif:
-  semax_body BtreeIndexVprog btrees_spec.Gprog f_RL_MoveToNext move_to_next_funspec.
-Proof. 
-  eapply semax_body_funspec_sub.
-  2: eapply sub_move_to_next.
-  apply body_RL_MoveToNext.
-  simpl.
-  assert (K: list_norepet [_t'3]). 
-  apply list_norepet_cons. 2: apply list_norepet_nil.
-  inversion 1. assert (M: list_norepet[_t'1; _t'3]).
-  apply list_norepet_cons; auto. inversion 1.
-  inversion H0. inversion H0.
-  assert (N: list_norepet [_t'2; _t'1; _t'3]).
-  apply list_norepet_cons; auto. 
-  inversion 1.
-  inversion H0. inversion H0. inversion H1. inversion H1.
-  apply list_norepet_cons; auto. 
-  inversion 1.
-  inversion H0. inversion H0. inversion H1. inversion H1.
-  inversion H2. inversion H2.
-Qed.
-
-Lemma move_to_previous_verif:
-    semax_body BtreeIndexVprog btrees_spec.Gprog f_RL_MoveToPrevious move_to_previous_funspec.
+Definition BtreeIndexVSU: @VSU NullExtension.Espec BtreeVprog _ 
+      nil imported_specs prog BtreeIndexASI.
 Proof.
-  eapply semax_body_funspec_sub.
-  2: eapply sub_move_to_previous.
-  apply body_RL_MoveToPrevious.
-  simpl.
-  assert (K: list_norepet [_t'1]). 
-  apply list_norepet_cons. 2: apply list_norepet_nil.
-  inversion 1.
-  apply list_norepet_cons; auto. 
-  inversion 1.
-  inversion H0. inversion H0.
+  eapply VSU_Exports_sub.
+  eapply BtreeVSU.
+  LNR_tac.
+  inversion 1. repeat if_tac in H1; subst.
+  all: inversion H1; subst; clear H1.
+  + exists (snd btrees_spec.RL_NumRecords_spec).
+      split. auto. apply sub_cardinality.
+  + exists (snd btrees_spec.RL_NewCursor_spec).
+      split. auto. apply sub_create_cursor.
+  + exists (snd btrees_spec.RL_NewRelation_spec).
+      split. auto. apply sub_create_index.
+  + exists (snd btrees_spec.RL_MoveToNext_spec).
+      split. auto. apply sub_move_to_next.
+  + exists (snd btrees_spec.RL_MoveToPrevious_spec).
+      split. auto. apply sub_move_to_previous.
+  + exists (snd btrees_spec.goToKey_spec).
+      split. auto. apply sub_go_to_key.
+  + exists (snd btrees_spec.RL_MoveToFirst_spec).
+      split. auto. apply sub_move_to_first.
+  + exists (snd btrees_spec.RL_GetRecord_spec).
+      split. auto. apply sub_get_record.
+  + exists (snd btrees_spec.RL_PutRecord_spec).
+      split. auto. apply sub_put_record.
 Qed.
-
-Lemma move_to_first_verif:
-  semax_body BtreeIndexVprog btree_wrappers.Gprog f_RL_MoveToFirst move_to_first_funspec.
-Proof. 
-  eapply semax_body_funspec_sub.
-  2: eapply sub_move_to_first.
-  apply body_RL_MoveToFirst.
-  simpl.
-  assert (K: list_norepet [_t'2]). 
-  apply list_norepet_cons. 2: apply list_norepet_nil.
-  inversion 1. assert (M: list_norepet[_t'3; _t'2]).
-  apply list_norepet_cons; auto. inversion 1.
-  inversion H0. inversion H0.
-  assert (N: list_norepet [_t'1; _t'3; _t'2]).
-  apply list_norepet_cons; auto. 
-  inversion 1.
-  inversion H0. inversion H0. inversion H1. inversion H1.
-  apply list_norepet_cons; auto. 
-  inversion 1.
-  inversion H0. inversion H0. inversion H1. inversion H1.
-  inversion H2. inversion H2.
-Qed.
-
-
-Lemma go_to_key_verif:
-  semax_body BtreeIndexVprog btrees_spec.Gprog f_goToKey go_to_key_funspec.
-Proof.
-  eapply semax_body_funspec_sub.
-  2: eapply sub_go_to_key.
-  apply body_goToKey.
-  simpl.
-  assert (K: list_norepet [_t'2]). 
-  apply list_norepet_cons. 2: apply list_norepet_nil.
-  inversion 1. assert (M: list_norepet[_t'1; _t'2]).
-  apply list_norepet_cons; auto. inversion 1.
-  inversion H0. inversion H0.
-  assert (N: list_norepet [_key; _t'1; _t'2]).
-  apply list_norepet_cons; auto. 
-  inversion 1.
-  inversion H0. inversion H0. inversion H1. inversion H1.
-  apply list_norepet_cons; auto. 
-  inversion 1.
-  inversion H0. inversion H0. inversion H1. inversion H1.
-  inversion H2. inversion H2.
-Qed.
-
-
-Lemma get_record_verif:
-  semax_body BtreeIndexVprog btrees_spec.Gprog f_RL_GetRecord get_record_funspec.
-Proof.
-  eapply semax_body_funspec_sub.
-  2: eapply sub_get_record.
-  apply body_RL_GetRecord.
-  simpl.
-  assert (K: list_norepet [_t'6]). 
-  apply list_norepet_cons. 2: apply list_norepet_nil.
-  inversion 1. assert (M: list_norepet[_t'7; _t'6]).
-  apply list_norepet_cons; auto. inversion 1.
-  inversion H0. inversion H0.
-  assert (N: list_norepet [_t'1; _t'7; _t'6]).
-  apply list_norepet_cons; auto. 
-  inversion 1.
-  inversion H0. inversion H0. inversion H1. inversion H1.
-Admitted.
-
-Lemma put_record_verif:
-  semax_body BtreeIndexVprog btrees_spec.Gprog f_RL_PutRecord put_record_funspec.
-Proof.
-  eapply semax_body_funspec_sub.
-  2: eapply sub_put_record.
-  apply body_RL_PutRecord.
-  simpl.
-  assert (K: list_norepet [_record]). 
-  apply list_norepet_cons. 2: apply list_norepet_nil.
-  inversion 1. assert (M: list_norepet[_key; _record]).
-  apply list_norepet_cons; auto. inversion 1.
-  inversion H0. inversion H0.
-  apply list_norepet_cons; auto. 
-  inversion 1.
-  inversion H0. inversion H0. inversion H1. inversion H1.
-Qed. 
-*)
-
-
 
 End BtreeIndex_Component.
